examples/cnf/lrup/README.md
@@ -5,6 +5,3 @@ Array-based implementation of the LRUP checker
 
 [lrupScript.sml](lrupScript.sml):
 Specification of an LRUP checker for CNF
-
-[lrup_cnfScript.sml](lrup_cnfScript.sml):
-Syntax and semantics of CNF in the DIMACS format
